# Volunteering vocabulary

## Namespaces
### Ontology Base URI
prefix id:              <https://id.volunteeringdata.io/>
prefix :                <https://id.volunteeringdata.io/schema/>

### Core W3C ontologies (OWL 2 reserved vocabulary)
prefix rdf:             <http://www.w3.org/1999/02/22-rdf-syntax-ns#>
prefix rdfs:            <http://www.w3.org/2000/01/rdf-schema#>
prefix owl:             <http://www.w3.org/2002/07/owl#>
prefix xsd:             <http://www.w3.org/2001/XMLSchema#>

### Other namespaces used
prefix dc:              <http://purl.org/dc/terms/>
prefix skos:            <http://www.w3.org/2004/02/skos/core#>
prefix time:            <http://www.w3.org/2006/time#>
prefix vann:            <http://purl.org/vocab/vann/>

## Concept Subclasses
:DigitalAccessibility
    a owl:Class ;
    rdfs:isDefinedBy id:schema ;
    rdfs:subClassOf :Accessibility ;
    rdfs:label "Digital Accessibility"@en ;
    rdfs:comment "Any accessbility information regarding digital requirements for an activity" ;"
.

:PhysicalAccessibility
    a owl:Class ;
    rdfs:isDefinedBy id:schema ;
    rdfs:subClassOf :Accessibility ;
    rdfs:label "Physical Accessibility"@en ;
    rdfs: comment "Any accessbibility information regarding physical ability required for an activity" ;
.

## Accessibility Concepts
[
    a :Accessibility ;
    rdfs:label "Expenses Paid" ;
    rdfs:comment "Any information regarding reimbursement for activity or role-related expenses.";
] .

[
    a :Accessibility ;
    rdfs:label "Age Requirements" ;
    rdfs:comment "Any information regarding specific ages or ranges of ages required or disallowed from a activity." ;
] .

[
    a :Accessibility ;
    rdfs:label "Language Requirements" ;
    rdfs:comment "Any language information for an activity, including required language(s) and translation services available." ;
] .

##Physical Accessibility Concepts
[
    rdfs:subClassOf :PhysicalAccessibility ;
    rdfs:label "Remote Accessibility" ;
    rdfs:comment "Any accomodations available for remote participation in an activity." ;

[
    rdfs:subClassOf :PhysicalAccessibility ;
    rdfs:label "Building Accessibility Features" ;
    rdfs:comment "Any information on building accessibility features for mobility aid users and accessible gender, faith, etc. rooms." ;
] .

[
    rdfs:subClassOf :PhysicalAccessibility ;
    rdfs:label "Public Transport Access" ;
    rdfs:comment "Any information on venue access via public transport lines." ;
] .

[
    rdfs:subClassOf :PhysicalAccessibility ;
    rdfs:label "Parking Availability" ;
    rdfs:comment "Any information on parking availability and accessibility at the venue." ;
] .

[
    rdfs:subClassOf :PhysicalAccessibility ;
    rdfs:label "Service Animals" ;
    rdfs:comment "Accessiblity information regarding usage of service animals in and around venue." ;
] .

[
    rdfs:subClassOf :PhysicalAccessibility ;
    rdfs:label "Visual Impairment" ;
    rdfs:comment "Any information on activities wherin visual impairments may be affected or accommodated." ;
] .

[
    rdfs:subClassOf :PhysicalAccessibility ;
    rdfs:label "Care Professionals" ;
    rdfs:comment "Any accommodations available for volunteers assisted by care professionals." ;
] .

##Digital Accessibility Concepts
[
    rdfs:subClassOf :DigitalAccessibility ;
    rdfs:label "Wifi Usage" ;
    rdfs:comment "Any information on wifi usage necessary for a activity." ;
] .

[
    rdfs:subClassOf :DigitalAccessibility ;
    rdfs:label "Technology Requirements" ;
    rdfs:comment "Any information on devices (laptop, phone, smartphone) and software required for a activity." ;
] .

[
    rdfs:subClassOf :DigitalAccessibility ;
    rdfs:label "Technology Availability" ;
    rdfs:comment "Any information on supplementory accessiblity software available in activities (screen readers, captioning)." ;
] .
